nondeterministic prelude except for soundness; reduction for propositional rules

theories/L/Complexity/Cook/GenNP.v
@@ -1,10 +1,20 @@
 From Undecidability.TM Require Import TM.
 From Undecidability.L.TM Require Import TMflat TMflatEnc TMflatFun TMEncoding TapeDecode TMunflatten.
 
-Definition mkinitTape (sig : finType) (i : list sig) : tape sig := match i with nil => niltape sig | (x::xr) => @leftof sig x xr end. 
+
+Definition isValidInput (sig : finType) k (s : list sig) := |s| <= k. 
+
+Definition initialTapeForString (sig : finType) (s : list sig) :=
+  match s with
+    | [] => niltape sig
+    | x::s => @leftof sig x s
+  end. 
 
 (*single-tape machine whose head will always start at the leftmost position (i.e. initial tapes are niltape or leftof) *)
-Definition GenNP : TM*nat*nat -> Prop:=
+Definition GenNPflat : TM*nat*nat -> Prop:=
   fun '(M,maxSize, steps (*in unary*)) =>
-    exists sig (M':mTM sig 1), isFlatteningTMOf M M' /\ (exists i, (exists f, loopM (initc M' ([|mkinitTape i|])) steps = Some f)
+    exists sig (M':mTM sig 1), isFlatteningTMOf M M' /\ (exists i, (exists f, loopM (initc M' ([|initialTapeForString i|])) steps = Some f)
          /\ length i <= maxSize).
+
+Definition GenNP (i : { sig : finType & (mTM sig 1 * nat * nat)%type } ) : Prop := 
+  match i with existT _ sig (tm, k, t) => exists inp, |inp| <= k /\ exists f, loopM (initc tm ([|initialTapeForString inp|])) t = Some f end. 
